$$
\begin{eqnarray}
\text{dot product:} \\
\vec{u} \cdot \vec{v} = \vec{u}^T \cdot \vec{v} = \sum{u_i*v_i} = \|\vec{u}\|\|\vec{v}\|cos(\alpha)
= \begin{pmatrix} u_1, u_2, u_3 \end{pmatrix} \cdot
\begin{pmatrix} v_1 \\ v_2 \\ v_3 \end{pmatrix} \\
\neq 
\vec{u} \cdot \vec{v}^T =
\begin{pmatrix} u_1 \\ u_2 \\ u_3 \end{pmatrix} \cdot
\begin{pmatrix} v_1, v_2, v_3 \end{pmatrix} =
\begin{pmatrix} 
u_1v_1, u_1v_2, u_1v_3 \\
u_2v_1, u_2v_2, u_2v_3 \\
u_3v_1, u_3v_2, u_3v_3
\end{pmatrix} \\
\alpha = 0 \implies \vec{u} \parallel \vec{v} \implies \vec{u} \cdot \vec{v} = \|\vec{u}\|\|\vec{v}\| \\
\alpha = \frac{\pi}{2} \implies \vec{u} \perp \vec{v} \implies \vec{u} \cdot \vec{v} = 0 \\
\text{dot product properties} \\
\text{commutative: } \vec{u}^T \cdot \vec{v} = \vec{v}^T \cdot {v} \\
\text{distributive: } \vec{u}^T \cdot (\vec{v} + \vec{w}) = \vec{u}^T \cdot \vec{v} + \vec{u}^T \cdot \vec{w}
\end{eqnarray} 
$$



